theories/Spilling/StupSpill.v
@@ -1,102 +1,139 @@
 Require Import List Map Env AllInRel Exp.
 Require Import IL Annotation InRel AutoIndTac Liveness LabelsDefined.
-Require Import SimI.
 Require Import Spilling.
 
 
-Fixpoint stupSpill (R : set var) (s : stmt) (Lv : ann (set var))
-: ann (set var * set var * option (list (set var * set var))) :=
-match s,Lv with
-| stmtLet x e t, ann1 LV lv => ann1 (R, Exp.freeVars e, None)
-                        (stupSpill (singleton x) t lv)
-| stmtReturn e, _ => ann0 (∅, Op.freeVars e, None)
-| stmtIf e t v, ann2 LV lv_s lv_t => ann2 (R, Op.freeVars e, None)
-                       (stupSpill (Op.freeVars e) t lv_s)
-                       (stupSpill (Op.freeVars e) v lv_t)
-| stmtApp f Y, _  => ann0 (R, list_union (Op.freeVars ⊝ Y), None)
-| stmtFun F t, annF LV als lv_t =>
-    annF (R, ∅, Some (List.map (fun lv => (∅, lv)) (List.map getAnn als)))
-           (zip (fun Zs lv => stupSpill ∅ (snd Zs) lv) F als)
-           (stupSpill ∅ t lv_t)
-| _,_ => ann0 (∅, ∅, None)
-end.
+Fixpoint stupSpill
+         (R : ⦃var⦄)
+         (s : stmt)
+         (Lv : ann (⦃var⦄))
+  : spilling
+  :=
+    match s,Lv with
+    | stmtLet x e t, ann1 LV lv
+      => ann1 (R, Exp.freeVars e, None) (stupSpill (singleton x) t lv)
+
+    | stmtReturn e, _
+      => ann0 (R, Op.freeVars e, None)
+
+    | stmtIf e t v, ann2 LV lv_s lv_t
+      => ann2 (R, Op.freeVars e, None) (stupSpill (Op.freeVars e) t lv_s)
+                                       (stupSpill (Op.freeVars e) v lv_t)
+
+    | stmtApp f Y, _
+      => ann0 (R, ∅, Some (inr (list_union (Op.freeVars ⊝ Y))))
+
+    | stmtFun F t, annF LV als lv_t
+      => annF (R, ∅, Some (inl ((fun lv => (∅, lv)) ⊝ getAnn ⊝ als)))
+              ((fun Zs lv => stupSpill ∅ (snd Zs) lv) ⊜ F als)
+              (stupSpill ∅ t lv_t)
+
+    | _,_ => ann0 (∅, ∅, None)
+
+    end
+.
 
 
-Lemma stupSpill_sat_spillSound (k:nat) (s:stmt) (R R' M : set var)
-  (Λ : list (set var * set var)) (Lv : list (set var)) (ZL : list params)
-  (alv : ann (set var)) :
-k > 0
--> R [=] R'
--> getAnn alv ⊆ R ∪ M
--> fv_e_bounded k s
--> live_sound Imperative ZL Lv s alv
--> PIR2 (fun RMf G => fst RMf [=] ∅ /\ snd RMf [=] G) Λ Lv
--> spill_sound k ZL Λ (R,M) s (stupSpill R' s alv).
 
+Lemma stupSpill_sat_spillSound
+      (k:nat)
+      (s:stmt)
+      (R R' M : ⦃var⦄)
+      (Λ : list (⦃var⦄ * ⦃var⦄))
+      (Lv : list ⦃var⦄)
+      (ZL : list params)
+      (alv : ann ⦃var⦄)
+  :
+    k > 0
+    -> R [=] R'
+    -> getAnn alv ⊆ R ∪ M
+    -> fv_e_bounded k s
+    -> live_sound Imperative ZL Lv s alv
+    -> PIR2 (fun RMf G => fst RMf [=] ∅ /\ snd RMf [=] G) Λ Lv
+    -> spill_sound k ZL Λ (R,M) s (stupSpill R' s alv)
+.
 Proof.
-intros kgeq1 ReqR' fvRM fvBound lvSound pir2.
-general induction lvSound;
-  inversion_clear fvBound
-    as [k0 x0 e0 s0 fvBcard fvBs
-       |k0 e0 fvBcard
-       |k0 e0 s0 t0 fvBcard fvBs fvBt
-       |k0 f0 Y0
-       |k0 Z0 s0 t0 fvBs fvBt];
-  simpl in *.
+  intros kgeq1 ReqR' fvRM fvBound lvSound pir2.
+  general induction lvSound;
+    inversion_clear fvBound
+      as [k0 x0 e0 s0 fvBcard fvBs
+         |k0 e0 fvBcard
+         |k0 e0 s0 t0 fvBcard fvBs fvBt
+         |k0 f0 Y0
+         |k0 Z0 s0 t0 fvBs fvBt];
+    simpl in *.
 
-- eapply SpillLet with (K:= R) (Kx := Exp.freeVars e).
-  + assert (seteq : singleton x [=] {x; (R\R ∪Exp.freeVars e) \Exp.freeVars e}).
-    { cset_tac. }
-    eapply IHlvSound; eauto with cset.
-    * rewrite seteq. reflexivity.
-    * rewrite <- seteq. rewrite <- ReqR'. rewrite <- fvRM.
-      rewrite <- H0. clear. cset_tac.
-      decide (x === a); eauto with cset.
-  + cset_tac.
-  + assert (seteq : R \ R ∪ Exp.freeVars e [=] Exp.freeVars e).
-    { cset_tac. }
-    rewrite seteq. rewrite fvBcard. trivial.
-  + assert (seteq :{x; (R \ R ∪Exp.freeVars e)\ Exp.freeVars e} [=] singleton x).
-    { cset_tac. }
-    rewrite seteq. rewrite singleton_cardinal. omega.
-- eapply SpillIf with (K:= R).
-  + cset_tac.
-  + assert (seteq : R\R ∪ Op.freeVars e [=] Op.freeVars e). { cset_tac. }
-    rewrite seteq. rewrite fvBcard. trivial.
-  + eapply IHlvSound1; eauto with cset.
-    * cset_tac.
-    * rewrite <- ReqR'. rewrite <- fvRM. cset_tac.
-  + eapply IHlvSound2; eauto with cset.
-    * cset_tac.
-    * rewrite <- ReqR'. rewrite <- fvRM. cset_tac.
-- eapply PIR2_nth_2 with (l:=counted l) in pir2; eauto using zip_get.
-  destruct pir2 as [[R_f M_f] [pir2_get [pir2_R pir2_M]]]. simpl in *.
-  eapply SpillApp with (K:= R) (R_f:= R_f) (M_f:=M_f).
-  + assert (seteq : forall s, R \ R ∪ s [=] s). { cset_tac. }
-    rewrite seteq. eauto.
-  + eauto.
-  + eauto.
-  (* + simpl. eauto.*)
-  + rewrite pir2_R. clear. cset_tac.
-  + rewrite pir2_M. rewrite H1. rewrite <- ReqR'. eauto.
-- eapply SpillReturn with (K:= R).
-  + cset_tac.
-  + assert (seteq : R\R ∪ Op.freeVars e [=] Op.freeVars e). { cset_tac. }
-    rewrite seteq. rewrite fvBcard. trivial.
-- eapply SpillFun with (K:=R).
-  + assert (seteq : R \ R ∪ ∅ [=] ∅). { cset_tac. }
-    rewrite seteq. rewrite empty_cardinal. omega.
-  + symmetry. apply zip_length2. eauto.
-  + repeat rewrite Coqlib.list_length_map. assumption.
-  + intros ; inv_get. simpl. rewrite empty_cardinal. omega.
-  + intros ; inv_get. eapply H1; eauto.
-    eapply PIR2_app; eauto.
-    eapply PIR2_get; eauto with len.
-    intros ; inv_get. simpl. split; eauto with cset.
-  + eapply IHlvSound; eauto.
-    * cset_tac.
-    * rewrite <- ReqR'. rewrite H3. rewrite fvRM. clear. cset_tac.
-    * eapply PIR2_app; eauto.
+  - eapply SpillLet with (K:= R) (Kx := Exp.freeVars e);
+      [ rewrite <- ReqR' | rewrite <- ReqR' | | | | ]; eauto.
+    + rewrite <- fvRM.
+      apply Exp.freeVars_live; eauto.
+    + assert (seteq : singleton x [=] {x; (R\R ∪Exp.freeVars e) \Exp.freeVars e}).
+      { cset_tac. }
+      eapply IHlvSound; eauto with cset.
+      * rewrite seteq. reflexivity.
+      * rewrite <- seteq. rewrite <- ReqR'. rewrite <- fvRM.
+        rewrite <- H0. clear. cset_tac.
+        decide (x === a); eauto with cset.
+    + assert (seteq : R \ R ∪ Exp.freeVars e [=] Exp.freeVars e).
+      { cset_tac. }
+      rewrite seteq. rewrite fvBcard. trivial.
+    + assert (seteq :{x; (R \ R ∪Exp.freeVars e)\ Exp.freeVars e}
+                       [=] singleton x).
+      { cset_tac. }
+      rewrite seteq. rewrite singleton_cardinal. omega.
+  - eapply SpillIf with (K:= R);
+      [ rewrite <- ReqR' | rewrite <- ReqR' | | | | ]; eauto.
+    + rewrite <- fvRM.
+      apply Op.freeVars_live; eauto.
+    + assert (seteq : R\R ∪ Op.freeVars e [=] Op.freeVars e).
+      { cset_tac. }
+      rewrite seteq. rewrite fvBcard. trivial.
+    + eapply IHlvSound1; eauto with cset.
+      * cset_tac.
+      * rewrite <- ReqR'. rewrite <- fvRM. cset_tac.
+    + eapply IHlvSound2; eauto with cset.
+      * cset_tac.
+      * rewrite <- ReqR'. rewrite <- fvRM. cset_tac.
+  - eapply PIR2_nth_2 with (l:=counted l) in pir2; eauto using zip_get.
+    destruct pir2 as [[R_f M_f] [pir2_get [pir2_R pir2_M]]]. simpl in *.
+    eapply SpillApp with (K:= R) (R_f:= R_f) (M_f:=M_f);
+      [rewrite <- ReqR' | rewrite <- ReqR' | | | | | | | rewrite <- ReqR'];
+      eauto.
+    + cset_tac.
+    + assert (R \ R ∪ ∅ [=] ∅) by cset_tac.
+      rewrite H5.
+      rewrite empty_cardinal.
+      omega.
+    + rewrite pir2_R. clear. cset_tac.
+    + rewrite pir2_M. rewrite H1. rewrite <- ReqR'. eauto.
+    + apply list_union_incl; eauto with cset.
+      intros.
+      inv_get.
+      rewrite <- fvRM.
+      exploit H3; eauto.
+      apply Op.freeVars_live; eauto.
+  - eapply SpillReturn with (K:= R);
+      [ rewrite <- ReqR' | rewrite <- ReqR' | | ]; eauto with cset.
+    + rewrite <- fvRM.
+      apply Op.freeVars_live; eauto.
+    + assert (seteq : R\R ∪ Op.freeVars e [=] Op.freeVars e) by cset_tac.
+      rewrite seteq. rewrite fvBcard. trivial.
+  - eapply SpillFun with (K:=R);
+    [ rewrite <- ReqR' | rewrite <- ReqR' | | | | | | ];
+      eauto with cset.
+    + assert (seteq : R \ R ∪ ∅ [=] ∅) by cset_tac.
+      rewrite seteq. rewrite empty_cardinal. omega.
+    + symmetry. apply zip_length2. eauto.
+    + repeat rewrite Coqlib.list_length_map. assumption.
+    + intros ; inv_get. simpl. rewrite empty_cardinal. omega.
+    + intros ; inv_get. eapply H1; eauto.
+      eapply PIR2_app; eauto.
       eapply PIR2_get; eauto with len.
       intros ; inv_get. simpl. split; eauto with cset.
+    + eapply IHlvSound; eauto.
+      * cset_tac.
+      * rewrite <- ReqR'. rewrite H3. rewrite fvRM. clear. cset_tac.
+      * eapply PIR2_app; eauto.
+        eapply PIR2_get; eauto with len.
+        intros ; inv_get. simpl. split; eauto with cset.
 Qed.
